\chapter{Fundamentals}

\section{Parse Tree}
Admit.


\section{Parsing and Precedence}
Admit.


\section{Lambda Calculus Reduction}
$(\lambda x.xy)$


\section{Symbolic Evaluation}
\begin{enumerate}
  \item Normal order: \\
  \begin{tabular}{rl}
      & $((\lambda f.\lambda g.f(g(1)))(\lambda x.x+4))(\lambda y.3-y)$ \\
    = & $(\lambda g.((\lambda x.x+4)(g\ 1)))(\lambda y.3-y) $ \\
    = & $(\lambda g.((g\ 1)+4))(\lambda y.3-y) $ \\
    = & $((\lambda y.3-y)\ 1)+4$ \\
    = & $(3-1)+4$ \\
  \end{tabular}

  \item Applicative order: \\
  \begin{tabular}{rl}
      & $((\lambda f.\lambda g.f(g(1)))(\lambda x.x+4))(\lambda y.3-y)$ \\
    = & $(\lambda g.((\lambda x.x+4)(g\ 1)))(\lambda y.3-y) $ \\
    = & $(\lambda x.x+4)((\lambda y.3-y)\ 1)$ \\
    = & $(\lambda x.x+4)(3-1)$ \\
    = & $(3-1)+4$ \\
  \end{tabular}
\end{enumerate}


\section{Lambda Reduction with Sugar}
Admit.


\section{Translation into Lambda Calculus}
\begin{tabular}{rl}
   $f$ & $ = \lambda g.gg $ \\
  $ff$ & $ = (\lambda g.gg)(\lambda g.gg) $ \\
       & $ = (\lambda g.gg)(\lambda g.gg) $ \\
       & \ldots \\
\end{tabular}


\section{Order of Evaluation}
Admit.


\section{Denotational Semantics}
\begin{enumerate}
  \item \ \\
  \begin{tabular}{rl}
      & $ C[[x:=1;\ x:=x+1]](s_{0}) $ \\
    = & $ C[[x:=x+1]](C[[x:=1]](s_{0})) $ \\
    = & $ C[[x:=x+1]](modify(s_{0}, x, E[[1]](s_{0}))) $ \\
    = & $ C[[x:=x+1]](modify(s_{0}, x, 1)) $ \\
    = & $ C[[x:=x+1]](s_{1}) $ \\
    = & $ modify(s_{1}, x, E[[x+1]](s_{1})) $ \\
    = & $ modify(s_{1}, x, E[[x]](s_{1}) + E[[1]](s_{1})) $ \\
    = & $ modify(s_{1}, x, 1+1) $ \\
  \end{tabular} \\
  where $ s_{1} = modify(s_{0}, x, 1) $.

  \item Admit.
\end{enumerate}


\section{Semantics of Initialize-Before-Use}
\begin{enumerate}
  \item \ \\
  \begin{tabular}{rl}
    & $ C[[x:=0;y:=0;if\ x=y\ then\ z:=0\ else\ w:=1]](s_{0}) $ \\
    = & $ C[[y:=0;if\ x=y\ then\ z:=0\ else\ w:=1]](C[[x:=0]](s_{0})) $ \\
    = & $ C[[y:=0;if\ x=y\ then\ z:=0\ else\ w:=1]](s_{1}) $ \\
    = & $ C[[if\ x=y\ then\ z:=0\ else\ w:=1]](C[[y:=0]](s_{1})) $ \\
    = & $ C[[if\ x=y\ then\ z:=0\ else\ w:=1]](s_{2}) $ \\
    = & $ if\ E[[x=y]](s_{2})\ then\ C[[z:=0]](s_{2})\ else\ C[[w:=1]](s_{2}) $ \\
    = & $ C[[z:=0]](s_{2}) $ \\
    = & $ if\ E[[0]](s_{2})=OK\ then\ modify(s_{2},z,init)\ else\ error $ \\
    = & $ modify(s_{2}, z, init) $ \\
  \end{tabular} \\

  \item \ \\
  \begin{tabular}{rl}
      & $ C[[if\ x=y\ then\ z:=y\ else\ z:=w]](s) $ \\
    = & $ if\ E[[x=y]]\ then\ C[[z:=y]](s)\ else\ C[[z:=w]](s) $ \\
    = & $ \ldots \ else\ if\ E[[w]]=OK\ then C[[z:=w]](s)\ else\ error $ \\
    = & $ \ldots \ else\ error $ \\
  \end{tabular}

\end{enumerate}


\section{Semantics of Type Checking}
Admit.


\section{Lazy Evaluation and Parallelism}
\begin{enumerate}
  \item Yes. While evaluating \texttt{g}, if we need the value of $\mathtt{e_{1}}$,
    which is not compeleted, we must wait.
  \item Admit.
  \item Admit.
  \item No.
\end{enumerate}
